Implement valid_instruction, make constructors respect binary

src/ast.v
@@ -2,6 +2,7 @@ Require Import util.
 
 Definition constant_bits := 32.
 Definition register_bits := 4.
+Definition nb_registers := 7.
 
 Inductive immediate: Type :=
 | imm: forall (i: N), immediate.
@@ -32,8 +33,8 @@ Inductive instruction: Type :=
 | nop: instruction
 | rrmovl: condition -> register -> register -> instruction
 | irmovl: immediate -> register -> instruction
-| rmmovl: register -> displacement -> register -> instruction
-| mrmovl: displacement -> register -> register -> instruction
+| rmmovl: register -> register -> displacement -> instruction
+| mrmovl: register -> register -> displacement -> instruction
 | OPl: operator -> register -> register -> instruction
 | jump: condition -> destination -> instruction
 | call: destination -> instruction
@@ -42,3 +43,21 @@ Inductive instruction: Type :=
 | popl: register -> instruction.
 
 Definition instructions := list instruction.
+Inductive valid_instruction (i: instruction): Type :=
+| valid_halt: i = halt -> valid_instruction i
+| valid_nop: i = nop -> valid_instruction i
+| valid_rrmovl: forall(c: condition)(n1 n2: nat),
+    n1 <= nb_registers -> n2 <= nb_registers -> i = (rrmovl c (reg (N.of_nat n1)) (reg (N.of_nat n2))) -> valid_instruction i
+| valid_irmovl: forall(imm: immediate)(n: nat),
+    n <= nb_registers -> i = (irmovl imm (reg (N.of_nat n))) -> valid_instruction i
+| valid_rmmovl: forall(n1: nat)(d: displacement)(n2: nat),
+    n1 <= nb_registers -> n2 <= nb_registers -> i = (rmmovl (reg (N.of_nat n1)) (reg (N.of_nat n2)) d) ->  valid_instruction i
+| valid_mrmovl: forall(d: displacement)(n1 n2: nat),
+    n1 <= nb_registers -> n2 <= nb_registers -> i = (mrmovl (reg (N.of_nat n1)) (reg (N.of_nat n2)) d) ->  valid_instruction i
+| valid_OPl: forall(o: operator)(n1 n2: nat),
+    n1 <= nb_registers -> n2 <= nb_registers -> i = (OPl o (reg (N.of_nat n1)) (reg (N.of_nat n2))) -> valid_instruction i
+| valid_jump: forall(c: condition)(d: destination), i = (jump c d) -> valid_instruction i
+| valid_call: forall(d: destination), i = (call d) -> valid_instruction i
+| valid_ret: i = ret -> valid_instruction i
+| valid_pushl: forall(n: nat), n < nb_registers -> i = (pushl (reg (N.of_nat n))) -> valid_instruction i
+| valid_popl:  forall(n: nat), n < nb_registers -> i = (popl (reg (N.of_nat n)))  -> valid_instruction i.
